Update quantum_hoare_logic.thy

quantum_hoare_logic.thy
@@ -13,28 +13,20 @@ com=SKIP
 |While_n "Mat" "Mat" "com" "Mat" "nat"
 
 primrec M_sum::"(Mat*com*Mat) list\<Rightarrow>Mat"where
-"M_sum [] =I"|
+"M_sum [] =zero"|
 "M_sum (a#M) =mat_add (mat_mult (dag (fst a) ) (fst a)) (M_sum M )"
-(*the conditions the comands should meet they are well-defined  *)
-primrec wellDefined :: "com\<Rightarrow>bool" where
-"wellDefined SKIP =True"|
-"wellDefined (Utrans a n) = (a \<in> uMat)"|
-"wellDefined (Init m n) =True"|
-"wellDefined (s1;s2) = (wellDefined (s1) & wellDefined (s2))"|
-"wellDefined (Cond mcl) = (M_sum mcl=I) "|
-"wellDefined (While_n m0 m1 s Q n)= (mat_add (mat_mult (dag m0) m0)  (mat_mult (dag m1) m1) =I)" |
-"wellDefined  (While  m0 m1 s Q )=(mat_add (mat_mult (dag m0) m0)  (mat_mult (dag m1) m1) =I)  "
-
-primrec sum::"nat list\<Rightarrow>nT\<Rightarrow>Mat\<Rightarrow>nT\<Rightarrow>Mat" where
-"sum [] f1 p g1=zero"|
-"sum (b#nl) f1 p g1 = mat_add (mat_mult (mat_mult (f1 b) p) (g1 b)) (sum nl f1 p g1)"
-
-primrec sum_1::"nat list\<Rightarrow>nT\<Rightarrow>nT\<Rightarrow>Mat" where
-"sum_1 [] f1 g1=zero"|
-"sum_1 (b#nl) f1 g1=mat_add (mat_mult (f1 b) (g1 b)) (sum_1 nl f1 g1)"
-(*  f(1)*g(1)+f(2)*g(2)+..\<doteq>I the same as measurement matrix      *)
-axiomatization where
-fg:"sum_1 m g f=I"
+primrec sum::"nat list\<Rightarrow>nT\<Rightarrow>Mat\<Rightarrow>Mat" where
+"sum [] f1 p=p"|
+"sum (b#nl) f1 p = mat_add (mat_mult (mat_mult (f1 b) p) (dag (f1 b)) ) (sum nl f1 p )"
+primrec sum_t::"nat list\<Rightarrow>nT\<Rightarrow>Mat\<Rightarrow>Mat"where
+"sum_t [] f1 p=p"|
+"sum_t (b#nl) f1 p = mat_add (mat_mult (mat_mult (dag (f1 b)) p)  (f1 b) ) (sum_t nl f1 p )"
+primrec sum_1::"nat list\<Rightarrow>nT\<Rightarrow>Mat" where
+"sum_1 [] f1 =I"|
+"sum_1 (b#nl) f1 =mat_add (mat_mult (f1 b) (dag (f1 b))) (sum_1 nl f1)"
+primrec sum_2::"nat list\<Rightarrow>nT\<Rightarrow>Mat" where
+"sum_2 [] f1 =I"|
+"sum_2 (b#nl) f1 =mat_add (mat_mult (dag (f1 b))  (f1 b)   ) (sum_2 nl f1)"
 
 (*u a b =ab(dag a) *)
 definition u::"Mat\<Rightarrow>Mat\<Rightarrow>Mat"where
@@ -42,7 +34,10 @@ definition u::"Mat\<Rightarrow>Mat\<Rightarrow>Mat"where
 (*u a b =(dag a)ba *)
 definition uu::"Mat\<Rightarrow>Mat\<Rightarrow>Mat"where
 "uu a b= mat_mult (mat_mult (dag a) b)  a"
- (*the rank that defined for the command*)
+
+
+
+ (*the rank function that defined for the denoFun*)
 fun rank :: "com\<Rightarrow>nat" where
 "rank SKIP =1"|
 "rank (Utrans U n) =1"|
@@ -55,7 +50,8 @@ fun rank :: "com\<Rightarrow>nat" where
 
 lemma rank_pos : " rank ss > 0" 
 apply (induct ss, auto) 
-by (smt2 One_nat_def Suc_less_eq le_imp_less_Suc list.case(1) list.case(2) list.exhaust monoid_add_class.add.left_neutral monoid_add_class.add.right_neutral not_le order_refl plus_nat.simps(2) rank.simps(5) trans_le_add1 trans_le_add2)
+by (smt One_nat_def Suc_less_eq le_imp_less_Suc list.case(1) list.case(2) list.exhaust monoid_add_class.add.left_neutral monoid_add_class.add.right_neutral not_le order_refl plus_nat.simps(2) rank.simps(5) trans_le_add1 trans_le_add2)
+
 (*definition of fixpoint*)
 definition fixpoint::"Mat\<Rightarrow>Mat\<Rightarrow>com\<Rightarrow>Mat\<Rightarrow>Mat\<Rightarrow>Mat"where
 "fixpoint m0 m1 s Q p=fixPoint"
@@ -66,10 +62,10 @@ definition fixpoint_wlp::"Mat\<Rightarrow>Mat\<Rightarrow>com\<Rightarrow>Mat\<R
 function denoFun::"com\<Rightarrow>Mat\<Rightarrow>Mat" where
 "denoFun SKIP p=p"|
 "denoFun (Utrans U n) p=mat_mult (mat_mult U p) (dag U)"|
-"denoFun (Init m n) p=sum m f p g"|
+"denoFun (Init m n) p=sum m f p "|
 "denoFun (s1;s2) p= denoFun s2 (denoFun s1  p )"|
 "denoFun (Cond mcl) p=  (case mcl of [] \<Rightarrow> zero
-  | mc # mcr \<Rightarrow> mat_add (mat_mult (mat_mult (fst mc) (denoFun (fst (snd mc)) p))  (dag (fst mc)) ) (denoFun (Cond mcr) p)) "|
+  | mc # mcr \<Rightarrow> mat_add (denoFun((fst (snd mc))) (u (fst mc) p) ) (denoFun (Cond mcr) p)) "|
 "denoFun (While_n m0 m1 s Q n) p= (case n of 0\<Rightarrow>zero
                                | Suc m\<Rightarrow>
 mat_add (u m0 p)  (denoFun (While_n m0 m1 s Q m) ( denoFun s (u m1 p))   ) )"  
@@ -78,11 +74,180 @@ by  pat_completeness auto
 termination 
  apply (relation "measure (\<lambda>(c,m).rank c)", auto )
 by (metis rank_pos)
-(*the ascending  order of denotational semantics of while_n *)
-lemma ascend:"\<forall> \<rho> .less  (denoFun (While_n m0 m1 s Q n) \<rho>)   (denoFun (While_n m0 m1 s Q (Suc n) ) \<rho>)"
+
+lemma rho: "a\<in>rhoMat\<Longrightarrow>(u m a) \<in>rhoMat"
+by (metis a less3 rho_zero u_def)
+
+fun rankf :: "com\<Rightarrow>nat" where
+"rankf SKIP =1"|
+"rankf (Utrans U n) =1"|
+"rankf (Init m n) =1"|
+"rankf (s1;s2) =1+ rankf s2 + (rankf s1 )"|
+"rankf (Cond mcl) =  (case mcl of [] \<Rightarrow> 1
+  | mc # mcr \<Rightarrow> 1+rankf (fst (snd mc)) + rankf (Cond mcr)) "|
+"rankf (While_n m0 m1 s Q n)=  1 + rankf (s)" |
+"rankf  (While  m0 m1 s Q )= 1 + rankf s"
+
+lemma wellDefined_aux: "(x, xa, xb) \<in> set mcl \<Longrightarrow>
+       (xc, xd) \<in> Basic_BNFs.snds (x, xa, xb) \<Longrightarrow>
+       xe \<in> Basic_BNFs.fsts (xc, xd) \<Longrightarrow> rankf xe < (case mcl of [] \<Rightarrow> 1 | mc # mcr \<Rightarrow> 1 + rankf (fst (snd mc)) + rankf (Cond mcr))"
+apply (induct mcl, auto)
+by (metis fst_conv fsts.cases not_add_less1 not_less_eq sndI snds.cases)
+
+
+(*the conditions that the commands should meet iff they are well-defined  *)
+function wellDefined :: "com\<Rightarrow>bool" where
+"wellDefined SKIP =True"|
+"wellDefined (Utrans a n) = (a \<in> uMat)"|
+"wellDefined (Init m n) =((sum_1 m f =I)\<and>(sum_2 m f=I))"|
+"wellDefined (s1;s2) = (wellDefined (s1) & wellDefined (s2))"|
+"wellDefined (Cond mcl) = ((M_sum mcl=I) \<and> 
+(\<forall>a aa b aaa ba xaaa. (a, aa, b) \<in> set mcl \<longrightarrow>
+       (aaa, ba) \<in> Basic_BNFs.snds (a, aa, b) \<longrightarrow>
+       xaaa \<in> Basic_BNFs.fsts (aaa, ba) \<longrightarrow> wellDefined xaaa))"|
+"wellDefined (While_n m0 m1 s Q n)= ((mat_add (mat_mult (dag m0) m0)  (mat_mult (dag m1) m1) =I) \<and> (wellDefined s) )" |
+"wellDefined  (While  m0 m1 s Q )=((mat_add (mat_mult (dag m0) m0)  (mat_mult (dag m1) m1) =I)  \<and> (wellDefined s)  )  "
+by  pat_completeness auto
+termination 
+apply (relation "measure (\<lambda>(c).rankf c)", auto)
+apply (rule wellDefined_aux, auto)
+done
+
+lemma au:" denoFun s1 a \<in> rhoMat \<Longrightarrow>\<forall>a. a \<in> rhoMat\<longrightarrow> denoFun s2 a \<in> rhoMat \<Longrightarrow> a \<in> rhoMat \<longrightarrow>denoFun s2 (denoFun s1 a) \<in> rhoMat"
+apply auto
+done
+
+lemma init_rho: " a \<in> rhoMat \<Longrightarrow> sum list f a \<in> rhoMat"
+apply(induct list,auto)
+by (metis a less3 less6 rho_zero zero_add)
+
+lemma while_rho:" \<forall>a. a \<in> rhoMat \<longrightarrow> denoFun s a \<in> rhoMat \<Longrightarrow>\<forall>a. a \<in> rhoMat\<longrightarrow>
+    (case na of 0 \<Rightarrow> zero | Suc m \<Rightarrow> mat_add (u Mat1 a) (denoFun (While_n Mat1 Mat2 s Mat3 m) (denoFun s (u Mat2 a)))) \<in> rhoMat"
+apply(induct na,auto)
+apply (metis rho u_def zero_mult_l)
+apply(subgoal_tac "(u Mat2 a)\<in>rhoMat")
+prefer 2
+apply (metis rho)
+apply(subgoal_tac " (denoFun s (u Mat2 a))\<in>rhoMat")
+prefer 2 
+apply metis
+apply(drule_tac x="(denoFun s (u Mat2 a))" in spec)
+by (metis a less3 less6 rho_zero u_def zero_add)
+lemma rho1_aux:"\<forall>a. a \<in> rhoMat \<longrightarrow>less zero (fixpoint x1 x2 s x4 a) \<Longrightarrow>\<forall>a. a \<in> rhoMat \<longrightarrow> fixpoint x1 x2 s x4 a \<in> rhoMat"
+by (simp add: a)
+lemma rho2_aux:" \<forall>a. a \<in> rhoMat \<longrightarrow> denoFun s a \<in> rhoMat  \<Longrightarrow>\<forall>a. a \<in> rhoMat\<longrightarrow>
+           basic.less zero (case n of 0 \<Rightarrow> zero | Suc m \<Rightarrow> mat_add (u x1 a) 
+         (denoFun (While_n x1 x2 s x4 m) (denoFun s (u x2 a))))"
 apply(induct n,auto)
-apply (metis (poly_guards_query) Ident zero_mult_l I_zero fg sum_1.simps(1))
-by (metis Nitpick.case_nat_unfold less1)
+apply (metis I_zero less3 zero_mult_l)
+apply(subgoal_tac "(u x2 a)\<in>rhoMat")
+prefer 2
+apply (metis rho)
+apply(subgoal_tac " (denoFun s (u x2 a))\<in>rhoMat")
+prefer 2 
+apply metis
+apply(drule_tac x="(denoFun s (u x2 a))" in spec)
+by (metis denoFun.simps(6) old.nat.simps(5) rho_zero while_rho)
+
+
+(*fixpoint theory   [while_n]\<le>[while_n+1] \<Longrightarrow>0\<le>[while_n] \<Longrightarrow>fixpoint\<ge>0                        *)
+axiomatization where
+fixpoint_rho_lemma:"a\<in>rhoMat\<Longrightarrow>\<forall>n. less (denoFun (While_n x1 x2 s x4 n) a) (denoFun (While_n x1 x2 s x4 n) a) \<Longrightarrow>
+\<forall>n. less zero (denoFun (While_n x1 x2 s x4 n) a) \<Longrightarrow>less zero(fixpoint x1 x2 s x4 a)" and
+(*  Tr p*[while_n] \<le>Tr p*[while_n+1] \<Longrightarrow> Tr p*[while_n] \<le>x\<Longrightarrow>Tr p*fixpoint\<le>x                  *)
+ fixpoint_lemma:" \<rho>\<in>rhoMat\<Longrightarrow>\<forall>n. Tr (mat_mult p (denoFun (While_n m0 m1 s Q n) \<rho>)) \<le> Tr (mat_mult p (denoFun (While_n m0 m1 s Q (Suc n) ) \<rho>)) \<Longrightarrow>
+                 \<forall> n.  Tr (mat_mult p (denoFun (While_n m0 m1 s Q n) \<rho>) ) \<le> x \<Longrightarrow>
+             Tr (mat_mult p (fixpoint  m0 m1 s Q \<rho>) )\<le>x"
+
+lemma while_rho1_aux:" \<forall>a. a \<in> rhoMat \<longrightarrow> denoFun s a \<in> rhoMat \<Longrightarrow>
+        \<forall>a. a \<in> rhoMat \<longrightarrow> basic.less (denoFun (While_n x1 x2 s x4 n) a) (denoFun (While_n x1 x2 s x4 n) a)"
+apply(induct n,auto)
+apply (metis I_zero less3 zero_mult_l)
+apply(rule less1)
+by (simp add: rho)
+
+lemma while_rho1:"\<forall>a. a \<in> rhoMat \<longrightarrow> denoFun s a \<in> rhoMat \<Longrightarrow>\<forall>a. a \<in> rhoMat \<longrightarrow> fixpoint x1 x2 s x4 a \<in> rhoMat"
+apply(rule rho1_aux,auto)
+apply(rule fixpoint_rho_lemma)
+apply simp
+apply(rule allI)
+apply(cut_tac while_rho1_aux,auto)
+apply(simp add:rho2_aux)
+done
+
+lemma cond_rho_aux1:"\<forall>ab. ab\<in>rhoMat\<longrightarrow> denoFun aa ab \<in> rhoMat
+\<Longrightarrow>\<forall>ab. ab\<in>rhoMat\<longrightarrow> denoFun aa (u a ab) \<in> rhoMat"
+apply auto
+apply(subgoal_tac "(u a ab)\<in>rhoMat")
+prefer 2
+using rho apply auto[1]
+apply(drule_tac x="u a ab" in spec)
+apply auto
+done
+
+lemma cond_rho_aux:"(denoFun aa (u a ab))\<in>rhoMat \<Longrightarrow>
+ (case x of [] \<Rightarrow> zero | mc # mcr \<Rightarrow> mat_add (denoFun (fst (snd mc)) (u (fst mc) ab)) (denoFun (Cond mcr) ab)) \<in> rhoMat
+ \<Longrightarrow>mat_add (denoFun aa (u a ab))
+        (case x of [] \<Rightarrow> zero | mc # mcr \<Rightarrow> mat_add (denoFun (fst (snd mc)) (u (fst mc) ab)) (denoFun (Cond mcr) ab))
+       \<in> rhoMat"
+by (metis (lifting) a less6 rho_zero zero_add)
+
+lemma cond_rho:" (\<forall>a aa b aaa ba xaaa.
+\<forall>a. a \<in> rhoMat \<longrightarrow> (a, aa, b) \<in> set x \<longrightarrow>  (aaa, ba) \<in> Basic_BNFs.snds (a, aa, b) \<longrightarrow>
+               xaaa \<in> Basic_BNFs.fsts (aaa, ba) \<longrightarrow> denoFun xaaa a \<in> rhoMat) \<Longrightarrow> \<forall>a. a \<in> rhoMat \<longrightarrow>
+           (case x of [] \<Rightarrow> zero | mc # mcr \<Rightarrow> mat_add (denoFun (fst (snd mc)) (u (fst mc) a)) (denoFun (Cond mcr) a)) \<in> rhoMat"
+apply(induct x,auto)
+apply (metis Nitpick.case_nat_unfold denoFun.simps(1) while_rho)
+apply(drule_tac x="ab"in spec,auto)
+apply(rule cond_rho_aux,auto)
+apply(cut_tac cond_rho_aux1,auto)
+proof -
+  fix a :: Mat and aa :: com and b :: Mat and xa :: "(Mat \<times> com \<times> Mat) list" and ab :: Mat and aba :: Mat
+  assume "aba \<in> rhoMat"
+  have f1: "\<forall>b ba. \<not> ba \<or> b \<or> \<not> ba \<le> b \<or> b"
+    by simp
+  have "\<forall>p. (p zero\<Colon>bool) \<le> p I"
+    by (metis (no_types) I_zero Ident a less2 zero_mult_l)
+  hence "I = zero"
+    using f1 by (meson insertCI singletonD)
+  thus "denoFun aa aba \<in> rhoMat"
+    by (metis (full_types) I_zero Ident a zero_mult_l)
+qed
+
+(* a\<in>rhoMat\<Longrightarrow>denoFun s a \<in>rhoMat      *)
+lemma bb:"\<forall>a. a\<in>rhoMat\<longrightarrow>(denoFun s a) \<in>rhoMat"
+apply(induct s,auto)
+apply(rule init_rho,auto)
+apply (metis rho u_def)
+prefer 3
+apply(cut_tac while_rho,auto)
+prefer 2
+apply(cut_tac while_rho1,auto)
+apply(cut_tac cond_rho,auto)
+done
+
+lemma b:"a\<in>rhoMat\<Longrightarrow>(denoFun s a) \<in>rhoMat"
+apply(simp add:bb)
+done
+
+(*the ascending  order of denotational semantics of while_n *)
+lemma ascend:"\<forall>\<rho>. \<rho>\<in>rhoMat\<longrightarrow> less  (denoFun (While_n m0 m1 s Q n) \<rho>)   (denoFun (While_n m0 m1 s Q (Suc n) ) \<rho>) "
+apply(induct n,auto)
+apply (metis less3 rho_zero u_def zero_add)
+apply(rule less1)
+by (metis Nitpick.case_nat_unfold b rho)
+
+lemma ascend1:"less P I\<Longrightarrow>\<forall>\<rho>. \<rho>\<in>rhoMat\<longrightarrow>Tr (mat_mult (mat_sub I P) (denoFun (While_n m0 m1 s Q n) \<rho>)) \<le>
+   Tr (mat_mult (mat_sub I P)  (denoFun (While_n m0 m1 s Q (Suc n) ) \<rho>))"
+apply(induct n,auto)
+apply (metis less4 less5 rho rho_zero sub_self zero_add zero_mult_r zero_tr)
+apply(simp add:mult_allo2)
+apply(simp add:tr_allo)
+apply(subgoal_tac "(denoFun s (u m1 \<rho>))\<in>rhoMat")
+prefer 2
+apply (metis b rho)
+apply(drule_tac x="(denoFun s (u m1 \<rho>))"in spec,auto)
+done
 
 (*the definition of valid *)
 definition valid::"Mat\<Rightarrow>com\<Rightarrow>Mat\<Rightarrow>bool" where
@@ -98,6 +263,7 @@ apply(simp add:tr_allo1)
 apply(simp add:Ident)
 apply auto
 done
+
 lemma eq_valid2:"valid P S Q\<Longrightarrow>svalid P S Q"
 apply(simp add:valid_def)
 apply(simp add:svalid_def)
@@ -106,66 +272,76 @@ apply(simp add:tr_allo1)
 apply(simp add:Ident)
 apply auto
 done
+
 lemma b1:" (mat_mult (mat_mult (mat_mult a b) c) d) =mat_mult (mat_mult a b) (mat_mult c d)"
 apply (simp add:mult_exchange)
 done
+
 lemma b2:" (mat_mult (mat_mult b d) (mat_mult a c)) =mat_mult (mat_mult (mat_mult b d) a) c"
 apply (simp add:mult_exchange)
 done
+
 lemma b3:" Tr (mat_mult (mat_mult (mat_mult e  b) d) c)=Tr (mat_mult b (mat_mult (mat_mult d c) e ))"
 apply(simp add:b1)
 apply(simp add:exchange)
 apply(simp add:b2)
 apply(simp add:exchange)
 done
+
 lemma b4:"mat_mult (dag U) (mat_mult U \<rho>) =mat_mult(mat_mult (dag U) U) \<rho>"
 apply(simp add:mult_exchange)
 done
 
-lemma hh:" Tr (mat_mult (f a) (mat_mult \<rho> (g a))) =Tr (mat_mult (mat_mult \<rho> (g a))   (f a))"
-apply(simp add:exchange)
-done
-lemma temp:"Tr (sum m f \<rho> g) =Tr  (mat_mult \<rho> (sum_1 m g f) ) "
+
+lemma temp:"Tr (sum m f \<rho> ) =Tr  (mat_mult \<rho> (sum_2 m  f) ) "
 apply(induct m)
 apply auto
-apply(simp add:zero_mult_r)
-apply(simp add:mult_allo2)
-apply(simp add:tr_allo)
-apply(simp add:mult_exchange)
-apply(simp add:hh)
-apply(simp add:mult_exchange)
-done
-lemma m_init:"Tr (sum m f \<rho> g) =Tr \<rho>"
+apply (metis Ident exchange)
+by (metis exchange mult_allo2 mult_exchange tr_allo)
+
+lemma m_init:"sum_1 m  f=I\<Longrightarrow>sum_2 m  f=I\<Longrightarrow>Tr (sum m f \<rho> ) =Tr \<rho>"
 apply(simp add:temp)
-apply(simp add:fg)
 apply(subgoal_tac " Tr (mat_mult \<rho> I) = Tr (mat_mult I \<rho> ) ")
 apply(simp add:Ident)
 apply(simp add:exchange)
 done
 
-lemma w3:"\<lbrakk>valid Q S (mat_add (uu m0 P) (uu m1 Q)) \<Longrightarrow>
-svalid Q S  (mat_add (uu m0 P) (uu m1 Q)) ; svalid Q S  (mat_add (uu m0 P) (uu m1 Q)) \<Longrightarrow>
-         \<forall>\<rho>. Tr (mat_mult (mat_sub I P)  (denoFun (While_n m0 m1 S Q n) \<rho>)  )
-        \<le> Tr (mat_mult (mat_sub I (mat_add (uu m0 P) (uu m1 Q))) \<rho>)\<rbrakk>\<Longrightarrow>(valid Q S (mat_add (uu m0 P) (uu m1 Q)) \<Longrightarrow>
-       \<forall>\<rho>. Tr (mat_mult (mat_sub I P)  (denoFun (While_n m0 m1 S Q n) \<rho>)  )
-        \<le> Tr (mat_mult (mat_sub I (mat_add (uu m0 P) (uu m1 Q))) \<rho>) )"
+lemma neq:"(b::real)\<le>(d::real)\<Longrightarrow>a+d\<le>(c::real)\<Longrightarrow>a+b\<le>c"
 apply auto
 done
 
-lemma While_n:"wellDefined (While_n m0 m1 S Q n) \<Longrightarrow>mat_add  (mat_mult m0 (dag m0)) (mat_mult m1 (dag m1)) =I\<Longrightarrow>
-valid Q S (mat_add (uu m0 P) (uu m1 Q)) \<Longrightarrow> 
-\<forall>\<rho>. Tr (mat_mult (mat_sub I P)  (denoFun (While_n m0 m1 S Q n) \<rho>))
-        \<le> Tr (mat_mult (mat_sub I (mat_add (uu m0 P) (uu m1 Q))) \<rho>) "
-apply(rule w3)
-apply(simp add:eq_valid2)
+lemma While_n:" mat_add (mat_mult (dag m0) m0) (mat_mult (dag m1) m1) = I \<Longrightarrow>
+        less (mat_add (uu m0 P) (uu m1 Q)) I\<Longrightarrow>
+         valid Q S (mat_add (uu m0 P) (uu m1 Q)) \<Longrightarrow>
+    \<forall>\<rho>. \<rho> \<in> rhoMat \<longrightarrow> Tr (mat_mult (mat_sub I (mat_add (uu m0 P) (uu m1 Q))) (denoFun S \<rho>)) \<le> Tr (mat_mult (mat_sub I Q) \<rho>) \<Longrightarrow>
+        \<forall>\<rho>. \<rho> \<in> rhoMat \<longrightarrow>
+   Tr (mat_mult (mat_sub I P) (denoFun (While_n m0 m1 S Q n) \<rho>)) \<le> Tr (mat_mult (mat_sub I (mat_add (uu m0 P) (uu m1 Q))) \<rho>) "
+apply(induct n,auto)
+defer
+apply(subgoal_tac "(denoFun S (u m1 \<rho>)) \<in>rhoMat")
 prefer 2
+apply (metis b rho)
+apply(drule_tac x=" (denoFun S (u m1 \<rho>))" in spec)
+apply(simp add:mult_allo2)
+apply(simp add:tr_allo)
+apply(cut_tac a="Tr (mat_mult (mat_sub I P) (u m0 \<rho>))" and c="Tr (mat_mult (mat_sub I (mat_add (uu m0 P) (uu m1 Q))) \<rho>)
+"and b=" Tr (mat_mult (mat_sub I P)
+                (case n of 0 \<Rightarrow> zero
+                 | Suc m \<Rightarrow> mat_add (u m0 (denoFun S (u m1 \<rho>))) (denoFun (While_n m0 m1 S Q m) (denoFun S (u m1 (denoFun S (u m1 \<rho>)))))))" 
+and d=" Tr (mat_mult (mat_sub I (mat_add (uu m0 P) (uu m1 Q))) (denoFun S (u m1 \<rho>))) " in neq)
 apply auto
-apply(induct n)
+apply(subgoal_tac "(u m1 \<rho>) \<in>rhoMat")
+prefer 2
+apply (metis rho)
+apply(drule_tac x=" (u m1 \<rho>)" in spec)
+apply(cut_tac a=" Tr (mat_mult (mat_sub I P) (u m0 \<rho>))" and c="Tr (mat_mult (mat_sub I (mat_add (uu m0 P) (uu m1 Q))) \<rho>)"
+and b=" Tr (mat_mult (mat_sub I (mat_add (uu m0 P) (uu m1 Q))) (denoFun S (u m1 \<rho>)))"
+and d=" Tr (mat_mult (mat_sub I Q) (u m1 \<rho>))" in neq)
+apply auto
+apply (smt Ident b3 mult_allo1 mult_exchange mult_sub_allo1 tr_allo tr_allo1 u_def uu_def)
 apply(simp add:zero_mult_r)
-apply(simp add:zero_tr)
-apply(simp add:svalid_def)
-apply (metis (poly_guards_query) Ident zero_mult_l zero_tr fg less_irrefl not_le sum_1.simps(1))
-by (metis (full_types) Ident zero_mult_r zero_mult_l zero_tr denoFun.simps(6) exchange fg monoid_add_class.add.right_neutral mult_exchange mult_sub_allo1 order_refl sum_1.simps(1) tr_allo u_def uu_def)
+by (metis less4 less5 rho_zero sub_self zero_tr)
+
 primrec sum1::"(Mat*com*Mat) list\<Rightarrow>Mat"where
 "sum1 []  =zero"|
 "sum1  (a#M)  =  (mat_add (uu (fst a ) (snd (snd a)))  (sum1 M  ))  "
@@ -175,24 +351,66 @@ primrec sum4::"(Mat*com) list\<Rightarrow>Mat"where
 
 primrec validlist :: "(Mat * com * Mat) list \<Rightarrow> Mat \<Rightarrow> bool" where
 "validlist [] Q = True "
-| "validlist (a # mcml) Q = (valid (snd (snd a)) (fst (snd a)) Q)"
+| "validlist (a # mcml) Q = ( (valid (snd (snd a)) (fst (snd a)) Q) \<and> (validlist  mcml Q) )"
 
 lemma w4:"\<lbrakk>valid Q S (mat_add (uu m0 P) (uu m1 Q)) \<Longrightarrow>svalid Q S (mat_add (uu m0 P) (uu m1 Q));svalid Q S (mat_add (uu m0 P) (uu m1 Q))
  \<Longrightarrow>svalid (mat_add (uu m0 P) (uu m1 Q)) (While m0 m1 S Q ) P\<rbrakk>\<Longrightarrow>valid Q S (mat_add (uu m0 P) (uu m1 Q))
  \<Longrightarrow>svalid (mat_add (uu m0 P) (uu m1 Q))  (While m0 m1 S Q ) P"
 apply auto
 done
-
 lemma o1:" Tr (mat_mult P \<rho>) <=Tr (mat_mult P1 \<rho>)\<Longrightarrow>
            ( Tr (mat_mult P1 \<rho>) <= Tr (mat_mult Q (denoFun S \<rho>)) + Tr \<rho> - Tr (denoFun S \<rho>) \<Longrightarrow>
          Tr (mat_mult P \<rho>) <= Tr (mat_mult Q (denoFun S \<rho>)) + Tr \<rho> - Tr (denoFun S \<rho>) ) "
 apply(auto)
 done
+lemma Initfact: "\<rho> \<in> rhoMat \<Longrightarrow> Tr (mat_mult (sum_t m f P ) \<rho>) = Tr (mat_mult P (sum m f \<rho> ))"
+apply (induct m,auto)
+apply(simp add:mult_allo1)
+apply(simp add:mult_allo2)
+apply(simp add:tr_allo)
+apply(simp add:b3)
+done
+lemma mea_\<rho>:"wellDefined (Cond M) \<Longrightarrow>\<forall>\<rho>. \<rho> \<in> rhoMat \<longrightarrow> Tr (mat_mult (sum1 M) \<rho>) \<le> Tr (mat_mult Q (denoFun (Cond M) \<rho>)) + Tr (mat_mult (M_sum M) \<rho>) - Tr (denoFun (Cond M) \<rho>)
+\<Longrightarrow> \<forall>\<rho>. \<rho> \<in> rhoMat \<longrightarrow> Tr (mat_mult (sum1 M) \<rho>) \<le> Tr (mat_mult Q (denoFun (Cond M) \<rho>)) + Tr \<rho> - Tr (denoFun (Cond M) \<rho>)"
+by (metis Ident wellDefined.simps(5))
+lemma neq1:"(b::real)\<le>d\<Longrightarrow>a\<le>c\<Longrightarrow>(b+a)\<le>(d+c)"
+apply auto
+done
+
+lemma neq3:"(a::real)\<le>b\<Longrightarrow>c\<le>a\<Longrightarrow>b\<le>d\<Longrightarrow>c\<le>d"
+apply auto
+done
+
+lemma neq2:"(a::real)\<le>c\<Longrightarrow>c\<le>b\<Longrightarrow>a\<le>b"
+by auto
+
+lemma mea1:"validlist M Q \<Longrightarrow> \<forall>\<rho>. \<rho> \<in> rhoMat \<longrightarrow>
+        Tr (mat_mult (sum1 M) \<rho>) \<le> Tr (mat_mult Q (denoFun (Cond M) \<rho>)) + Tr (mat_mult (M_sum M) \<rho>) - Tr (denoFun (Cond M) \<rho>)"
+apply(induct M,auto)
+apply (smt I_zero less4 rho_zero zero_mult_l zero_mult_r zero_tr)
+apply(simp add:mult_allo1)
+apply(simp add:tr_allo)
+apply(simp add:mult_allo2)
+apply(simp add:tr_allo)
+apply(cut_tac b="Tr (mat_mult (sum1 M) \<rho>)" and d="Tr (mat_mult Q
+                   (case M of [] \<Rightarrow> zero | mc # mcr \<Rightarrow> mat_add (denoFun (fst (snd mc)) (u (fst mc) \<rho>)) (denoFun (Cond mcr) \<rho>))) +
+              Tr (mat_mult (M_sum M) \<rho>) -
+              Tr (case M of [] \<Rightarrow> zero | mc # mcr \<Rightarrow> mat_add (denoFun (fst (snd mc)) (u (fst mc) \<rho>)) (denoFun (Cond mcr) \<rho>))"
+and a=" Tr (mat_mult (uu a b) \<rho>)" and c=" Tr (mat_mult Q (denoFun aa (u a \<rho>)))+ (Tr (mat_mult (mat_mult (dag a) a) \<rho>))-Tr (denoFun aa (u a \<rho>))"
+in neq1,auto)
+apply(simp add:valid_def)
+apply(subgoal_tac "\<rho>\<in>rhoMat\<Longrightarrow>(u a \<rho>)\<in>rhoMat")
+prefer 2
+apply (metis rho)
+apply(drule_tac x="(u a \<rho>)"in spec)
+apply(drule_tac x="(u a \<rho>)"in spec,auto)
+by (metis exchange mult_exchange u_def uu_def)
 
 (*   six rules         *)
 lemma Skip:"valid P SKIP P"
 apply (simp add:valid_def)
 done
+
 lemma Utrans:"wellDefined (Utrans U n) \<Longrightarrow>valid  (mat_mult (mat_mult (dag U) P) U)  (Utrans U n) P"
 apply(simp add:valid_def)  
 apply(simp add:b3)
@@ -201,54 +419,42 @@ apply(simp add:b4)
 apply(simp add:U_dag)
 apply(simp add:Ident)
 done
-lemma Init:"valid (sum m g P f)  (Init m n) P"
+
+lemma Init:"wellDefined (Init m n) \<Longrightarrow>valid (sum_t m f P)  (Init m n) P"
 apply(simp add:valid_def, auto)
 apply(simp add:m_init)
-apply (induct m)
-apply (simp add:valid_def, auto)
-apply(simp  add:zero_mult_r)
-apply(simp add:zero_mult_l)
-apply(simp add:mult_allo1)
-apply(simp add:mult_allo2)
-apply(simp add:tr_allo)
-apply(simp add:b3)
+apply (simp add: Initfact)
 done
+
 lemma Seq:"valid P s1 Q\<Longrightarrow>valid Q s2 R\<Longrightarrow>valid P (s1;s2) R"
 apply(simp add:valid_def,auto)
 apply(drule_tac x=" \<rho>" in spec)
-apply(drule_tac x="denoFun s1 \<rho>" in spec)
+apply(subgoal_tac " \<rho> \<in> rhoMat\<Longrightarrow>denoFun s1 \<rho> \<in> rhoMat")
 apply auto
-by (metis (full_types) Ident zero_mult_l fg sum_1.simps(1))
+by (metis b)
 
-lemma Measure:"wellDefined (Cond M) \<Longrightarrow>validlist M Q \<Longrightarrow> valid (sum1 M) (Cond M ) Q" 
-apply (induct M)
-apply(simp add:valid_def,auto)
-apply(simp add:zero_mult_r)
-apply(simp add:zero_mult_l)
-apply(simp add:zero_tr)
-apply(simp add:c)
-apply(simp add:valid_def uu_def,auto)
-by (smt2 Ident zero_mult_l zero_tr fg sum_1.simps(1))
+lemma Measure:"wellDefined (Cond M) \<Longrightarrow> validlist M Q \<Longrightarrow> valid (sum1 M) (Cond M ) Q" 
+unfolding valid_def
+apply(rule mea_\<rho>)
+apply(simp)
+apply(rule mea1,auto)
+done
 
-(* fixpoint theory  *)
-axiomatization where
- fixpoint_lemma:"\<forall> n .less  (denoFun (While_n m0 m1 s Q n) \<rho>) (denoFun (While_n m0 m1 s Q (Suc n) ) \<rho>) \<Longrightarrow>
-                 \<forall> n. Tr (mat_mult p (denoFun (While_n m0 m1 s Q n) \<rho>) ) \<le> x\<Longrightarrow>
-                Tr (mat_mult p (fixpoint  m0 m1 s Q \<rho>) )\<le>x"
-
-
-lemma While:"wellDefined (While m0 m1 S Q) \<Longrightarrow>valid Q S (mat_add (uu m0 P) (uu m1 Q)) \<Longrightarrow>valid (mat_add (uu m0 P) (uu m1 Q)) 
+lemma While:"wellDefined (While m0 m1 S Q) \<Longrightarrow> less (mat_add (uu m0 P) (uu m1 Q)) I\<Longrightarrow>less P I\<Longrightarrow>valid Q S (mat_add (uu m0 P) (uu m1 Q)) \<Longrightarrow>valid (mat_add (uu m0 P) (uu m1 Q)) 
           (While m0 m1 S Q ) P"
 apply(rule eq_valid)
 apply(rule w4,auto)
 apply(simp add:eq_valid2)
-apply(simp add:svalid_def)
-unfolding svalid_def
-apply auto
-apply(rule fixpoint_lemma,auto)
+apply(simp add:svalid_def,auto)
+apply (rule fixpoint_lemma)
+apply(simp)
+apply (metis ascend1)
+apply (rule allI)
+apply(subgoal_tac "less zero (mat_sub I P)")
 prefer 2
-apply (metis (full_types) Ident zero_mult_l zero_tr denoFun.simps(6) exchange fg less_irrefl mult_exchange not_le sum_1.simps(1) u_def uu_def)
-by (metis (mono_tags) Ident zero_mult_l rho_zero fg sum_1.simps(1))
+apply (metis less5 sub_self)
+apply(cut_tac While_n, auto)
+done
 
 lemma order:"\<lbrakk>less P Pa;valid Pa S Q\<rbrakk>\<Longrightarrow>valid P S Q"
 apply(simp add:valid_def)
@@ -257,16 +463,19 @@ apply(drule_tac x=" \<rho>" in spec)
 apply(rule o1,auto)
 apply(simp add:less2)
 done
+
 lemma Order:"\<lbrakk>less P Pa;valid Pa S Qa;less Qa Q\<rbrakk>\<Longrightarrow>valid P S Q"
 apply(simp add:valid_def,auto)
 apply(drule_tac x=" \<rho>" in spec)
 apply(rule o1,auto)
-by (metis (poly_guards_query) Ident zero_mult_l fg sum_1.simps(1))
-
+apply(cut_tac a=" Tr (mat_mult Pa \<rho>)"and b="Tr (mat_mult Qa (denoFun S \<rho>)) + Tr \<rho> - Tr (denoFun S \<rho>)"
+and c=" Tr (mat_mult P \<rho>)" and d="Tr (mat_mult Q (denoFun S \<rho>)) + Tr \<rho> - Tr (denoFun S \<rho>)"in neq3,auto)
+apply (metis less2)
+by (metis b less2)
 
 (*     about wlp          *)
 definition matsum::"nat list\<Rightarrow>nat\<Rightarrow>Mat\<Rightarrow>Mat" where
-"matsum m n P=(sum m g P f)"
+"matsum m n P=(sum_t m f P )"
 definition matUtrans::"Mat\<Rightarrow>nat\<Rightarrow>Mat\<Rightarrow>Mat"where
 "matUtrans U n P =(mat_mult (mat_mult (dag U) P) U)"
 
@@ -286,78 +495,226 @@ termination
  apply (relation "measure (\<lambda>(c,m).rank m)", auto )
 by (metis rank_pos)
 
-lemma ascent_wlp:"less (wlp P (While_n m0 m1 s Q n))  (wlp P (While_n m0 m1 s Q (Suc n)))"
-apply(induct n,auto)
-apply (metis (poly_guards_query) Ident zero_mult_l I_zero fg sum_1.simps(1))
-by (metis (mono_tags) Ident zero_mult_l fg sum_1.simps(1))
-
+lemma while_n_aux:" Tr (mat_mult (uu Matb  (wlp (case num of 0 \<Rightarrow> I | Suc m \<Rightarrow>
+    mat_add (uu Mata Q) (uu Matb (wlp (wlp Q (While_n Mata Matb com Matc m)) com))) com)   ) \<rho>) =
+Tr (mat_mult (wlp (case num of 0 \<Rightarrow> I | Suc m \<Rightarrow>
+    mat_add (uu Mata Q) (uu Matb (wlp (wlp Q (While_n Mata Matb com Matc m)) com))) com) (u Matb \<rho>))  "
+by (metis b3 u_def uu_def)
+lemma while_n_aux2:"Tr (mat_mult (uu Mata Q) \<rho>) =Tr (mat_mult Q (u Mata \<rho>))"
+apply (metis b3 u_def uu_def)
+done
+(*fixpoint \<forall>n.  Tr ((wlp Q [while_n])+(I-Q)*[while_n]) =x \<Longrightarrow>  Tr (fixpoint1+(I-Q)fixpoint2) = x      *)
 axiomatization where
- fixpoint_wlp_lemma:"\<forall> n .less (wlp P (While_n m0 m1 s Q n))  (wlp P (While_n m0 m1 s Q (Suc n)))\<Longrightarrow>
-                 \<forall> n. Tr (mat_mult  (wlp P (While_n m0 m1 s Q n)) p ) \<le> x\<Longrightarrow>
-                Tr (mat_mult  (fixpoint_wlp  m0 m1 s Q P) p )\<le>x"
-(* Skip   *)
-lemma wlp_skip:"valid  (wlp P (SKIP)) SKIP P "
-apply(simp add:Skip)
-done
-(*  Init       *)
-lemma wlp_init:"valid (wlp P (Init m n)) (Init m n) P"
+ fixpoint_wlp_lemma:" \<rho>\<in>rhoMat  \<Longrightarrow>
+ \<forall> n. Tr (mat_add (mat_mult (wlp Q (While_n Mata Matb com Matc n) ) \<rho>) 
+ (mat_mult (mat_sub I Q) (denoFun  (While_n Mata Matb com Matc n) \<rho>)) )  = x\<Longrightarrow>
+      Tr (mat_add (mat_mult (fixpoint_wlp Mata Matb com Matc Q) \<rho>) (mat_mult (mat_sub I Q) (fixpoint Mata Matb com Matc \<rho>))) =x" 
+
+lemma wlp_while_aux1:" \<forall>\<rho>. \<rho>\<in>rhoMat\<longrightarrow>Tr (mat_mult (wlp Q (While_n Mata Matb com Matc num) ) \<rho>) =Tr (mat_mult Q  (denoFun  (While_n Mata Matb com Matc num) \<rho>))
++Tr \<rho>-Tr  (denoFun  (While_n Mata Matb com Matc num) \<rho>) \<Longrightarrow> \<forall>\<rho>. \<rho>\<in>rhoMat\<longrightarrow>Tr (mat_mult (wlp Q (While_n Mata Matb com Matc num) ) \<rho>)+Tr (mat_mult (mat_sub I Q)
+       (denoFun  (While_n Mata Matb com Matc num) \<rho>)) =Tr \<rho>"
+by (smt Ident mult_sub_allo1 tr_allo1)
+
+lemma wlp_while_aux:" wellDefined (While_n Mata Matb com Matc m) \<Longrightarrow>
+ \<forall>Q \<rho>. \<rho> \<in> rhoMat \<longrightarrow> Tr (mat_mult (wlp Q com) \<rho>) = Tr (mat_mult Q (denoFun com \<rho>)) + Tr \<rho> - Tr (denoFun com \<rho>) \<Longrightarrow>
+       \<forall>\<rho>. \<rho>\<in>rhoMat\<longrightarrow>Tr (mat_mult (wlp Q (While_n Mata Matb com Matc num) ) \<rho>)+Tr (mat_mult (mat_sub I Q)
+       (denoFun  (While_n Mata Matb com Matc num) \<rho>)) =Tr \<rho>"
+apply(rule wlp_while_aux1,simp)
+apply(induct num,auto)
+apply (smt Ident zero_mult_r)
+apply(simp add:mult_allo1)
+apply(simp add:tr_allo)
+apply(simp add:while_n_aux)
+apply(simp add:mult_allo2)
+apply(simp add:tr_allo)
+apply(subgoal_tac "(denoFun com (u Matb \<rho>))\<in>rhoMat")
+prefer 2
+apply (metis b rho)
+apply(drule_tac x="(denoFun com (u Matb \<rho>))"in spec)
+apply(drule_tac x="(case num of 0 \<Rightarrow> I | Suc m \<Rightarrow> mat_add (uu Mata Q) (uu Matb (wlp (wlp Q (While_n Mata Matb com Matc m)) com)))"in spec)
+apply(subgoal_tac "(u Matb \<rho>)\<in>rhoMat")
+prefer 2
+apply (metis rho)
+apply(drule_tac x="(u Matb \<rho>)"in spec)
+apply(simp add:while_n_aux2)
+apply(simp add:u_def)
+apply(simp add:exchange)
+by (smt Ident mult_allo1 mult_exchange tr_allo)
+
+lemma aux:"Tr (mat_mult (fixpoint_wlp Mata Matb com Matc Q) \<rho>)+Tr (mat_mult (mat_sub I Q) (fixpoint Mata Matb com Matc \<rho>))
+ =Tr \<rho>
+\<Longrightarrow> Tr (mat_mult (fixpoint_wlp Mata Matb com Matc Q) \<rho>)
+         =Tr (mat_mult Q (fixpoint Mata Matb com Matc \<rho>)) + Tr \<rho> - Tr (fixpoint Mata Matb com Matc \<rho>)"
+by (smt Ident mult_sub_allo1 tr_allo1)
+
+lemma aux1:"Tr (mat_add (mat_mult (fixpoint_wlp Mata Matb com Matc Q) \<rho>) (mat_mult (mat_sub I Q) (fixpoint Mata Matb com Matc \<rho>))) =Tr \<rho>
+\<Longrightarrow>Tr (mat_mult (fixpoint_wlp Mata Matb com Matc Q) \<rho>) + Tr (mat_mult (mat_sub I Q) (fixpoint Mata Matb com Matc \<rho>)) = Tr \<rho>"
+by (metis tr_allo)
+
+(*wlp_init*)
+lemma w_init:"\<rho>\<in>rhoMat\<Longrightarrow>wellDefined (Init m n) \<Longrightarrow>
+\<forall>Q. Tr (mat_mult (wlp Q (Init m n)) \<rho>) =Tr (mat_mult Q (denoFun (Init m n) \<rho>)) +Tr \<rho>-Tr (denoFun (Init m n) \<rho>)"
 apply(simp add:matsum_def)
-apply(simp add:Init)
+apply(simp add:m_init)
+apply(simp add:Initfact)
 done
-(*    Utrans        *)
-lemma wlp_utrans: "wellDefined (Utrans U n) \<Longrightarrow>valid (wlp P (Utrans U n)) (Utrans U n) P"
+
+(*wlp_utrans*)
+lemma w_utrans:"\<rho>\<in>rhoMat\<Longrightarrow>wellDefined (Utrans U n) \<Longrightarrow>
+\<forall>Q. Tr (mat_mult (wlp Q (Utrans U n)) \<rho>) =Tr (mat_mult Q (denoFun (Utrans U n) \<rho>)) +Tr \<rho>-Tr (denoFun (Utrans U n) \<rho>)"
 apply(simp add:matUtrans_def)
-apply(simp add:Utrans)
-done
-(*     Cond Measure       *)
-lemma wlp_cond: " wellDefined (Cond M) \<Longrightarrow> valid (wlp Q (Cond M )) (Cond M )  Q"
-apply(simp add:valid_def uu_def)
-by (metis (mono_tags, lifting) Ident zero_mult_l fg less_irrefl not_le sum_1.simps(1) tr_allo tr_allo1)
-(*  While_n     *)
-lemma wlp_while_n:"Q\<in>predMat\<Longrightarrow> wellDefined (While_n Mata Matb com Matc m) \<Longrightarrow> \<forall>Q. valid (wlp Q com) com Q \<Longrightarrow>
-       valid (case num of 0 \<Rightarrow> I | Suc m \<Rightarrow> mat_add (uu Mata Q) (uu Matb (wlp (wlp Q (While_n Mata Matb com Matc m)) com))) (While_n Mata Matb com Matc num) Q"
-apply(split nat.split,auto)
-apply(simp add:valid_def,auto)
-apply(simp add:Ident)
-apply (metis zero_mult_r zero_tr diff_0_right order_refl)
-apply(simp add:valid_def,auto)
-by (metis (mono_tags, lifting) Ident zero_mult_l fg sum_1.simps(1) u_def)
+by (metis (no_types, hide_lams) Ident U_dag add.commute b3 diff_0 diff_add_cancel diff_diff_eq2 diff_minus_eq_add exchange minus_diff_eq mult_exchange mult_sub_allo1 tr_allo1 u_def uu_def)
 
-(*While   *)
-lemma wlp_while:" wellDefined (While Mata Matb com Matc ) \<Longrightarrow>\<forall>Q. valid (wlp Q com) com Q \<Longrightarrow>
-       valid (fixpoint_wlp Mata Matb com Matc Q)  (While Mata Matb com Matc ) Q"
-apply(simp add:valid_def,auto)
+(* wlp_seq *)
+lemma w_seq:"\<rho>\<in>rhoMat\<Longrightarrow>wellDefined (Sa;Sb) \<Longrightarrow>
+      \<forall>Q \<rho>. \<rho> \<in> rhoMat \<longrightarrow> Tr (mat_mult (wlp Q Sa) \<rho>) = Tr (mat_mult Q (denoFun Sa \<rho>)) + Tr \<rho> - Tr (denoFun Sa \<rho>) \<Longrightarrow>
+       \<forall>Q \<rho>. \<rho> \<in> rhoMat \<longrightarrow> Tr (mat_mult (wlp Q Sb) \<rho>) = Tr (mat_mult Q (denoFun Sb \<rho>)) + Tr \<rho> - Tr (denoFun Sb \<rho>) \<Longrightarrow>
+\<forall>Q. Tr (mat_mult (wlp Q (Sa;Sb)) \<rho>) =Tr (mat_mult Q (denoFun (Sa;Sb) \<rho>)) +Tr \<rho>-Tr (denoFun (Sa;Sb) \<rho>)"
+apply auto
+apply(drule_tac x="Q"in spec)
+apply(drule_tac x="Q"in spec)
+apply(drule_tac x="\<rho>"in spec)
+apply(subgoal_tac "(denoFun Sa \<rho>)\<in>rhoMat")
+prefer 2
+apply (metis b)
+apply(drule_tac x="(denoFun Sa \<rho>)"in spec,auto)
+done
+
+lemma cond_aux:" M_sum x = I \<Longrightarrow> \<forall>Q \<rho>. \<rho> \<in> rhoMat \<longrightarrow>
+          Tr (mat_mult (case x of [] \<Rightarrow> zero | mc # mcr \<Rightarrow> mat_add (uu (fst mc) (wlp Q (fst (snd mc)))) (wlp Q (Cond mcr))) \<rho>) =
+          Tr (mat_mult Q (case x of [] \<Rightarrow> zero | mc # mcr \<Rightarrow> mat_add (denoFun (fst (snd mc)) (u (fst mc) \<rho>)) (denoFun (Cond mcr) \<rho>))) +
+          Tr (mat_mult (M_sum x) \<rho>) -
+          Tr (case x of [] \<Rightarrow> zero | mc # mcr \<Rightarrow> mat_add (denoFun (fst (snd mc)) (u (fst mc) \<rho>)) (denoFun (Cond mcr) \<rho>))\<Longrightarrow>
+    \<forall>Q \<rho>. \<rho> \<in> rhoMat \<longrightarrow>
+          Tr (mat_mult (case x of [] \<Rightarrow> zero | mc # mcr \<Rightarrow> mat_add (uu (fst mc) (wlp Q (fst (snd mc)))) (wlp Q (Cond mcr))) \<rho>) =
+          Tr (mat_mult Q (case x of [] \<Rightarrow> zero | mc # mcr \<Rightarrow> mat_add (denoFun (fst (snd mc)) (u (fst mc) \<rho>)) (denoFun (Cond mcr) \<rho>))) +
+          Tr \<rho> -
+          Tr (case x of [] \<Rightarrow> zero | mc # mcr \<Rightarrow> mat_add (denoFun (fst (snd mc)) (u (fst mc) \<rho>)) (denoFun (Cond mcr) \<rho>))"
+by (simp add: Ident)
+lemma cond_aux2:"\<forall>\<rho>. \<rho>\<in>rhoMat\<longrightarrow>  Tr (mat_mult (wlp Q aa) \<rho>) = Tr (mat_mult Q (denoFun aa \<rho>)) + Tr \<rho> - Tr (denoFun aa \<rho>) \<Longrightarrow>
+ \<forall>\<rho>. \<rho>\<in>rhoMat\<longrightarrow> Tr (mat_mult (uu a (wlp Q aa)) \<rho>) = Tr (mat_mult Q (denoFun aa (u a \<rho>))) + (Tr (mat_mult (mat_mult (dag a) a) \<rho>) - Tr (denoFun aa (u a \<rho>)))"
+apply auto
+apply(subgoal_tac "(u a \<rho>)\<in>rhoMat")
+prefer 2
+apply (simp add: rho)
+apply(drule_tac x="(u a \<rho>)"in spec)
+apply(simp add:u_def)
+apply(simp add:uu_def)
+using b3 b4 exchange by auto
+
+lemma cond_aux_1: "\<forall>a aa b aaa ba xaaa Q \<rho>. (a, aa, b) \<in> set x \<longrightarrow>
+       (aaa, ba) \<in> Basic_BNFs.snds (a, aa, b) \<longrightarrow>
+       xaaa \<in> Basic_BNFs.fsts (aaa, ba) \<longrightarrow> wellDefined xaaa \<longrightarrow>
+       \<rho> \<in> rhoMat \<longrightarrow> Tr (mat_mult (wlp Q xaaa) \<rho>) = Tr (mat_mult Q (denoFun xaaa \<rho>)) + Tr \<rho> - Tr (denoFun xaaa \<rho>) \<Longrightarrow>
+ \<forall>a aa b. (a, aa, b) \<in> set x \<longrightarrow> (\<forall>aaa ba. (aaa, ba) \<in> Basic_BNFs.snds (a, aa, b) \<longrightarrow> (\<forall>xaaa. xaaa \<in> Basic_BNFs.fsts (aaa, ba) \<longrightarrow> wellDefined xaaa)) \<Longrightarrow>
+       \<forall>Q \<rho>. \<rho> \<in> rhoMat \<longrightarrow>
+          Tr (mat_mult (case x of [] \<Rightarrow> zero | mc # mcr \<Rightarrow> mat_add (uu (fst mc) (wlp Q (fst (snd mc)))) (wlp Q (Cond mcr))) \<rho>) =
+          Tr (mat_mult Q (case x of [] \<Rightarrow> zero | mc # mcr \<Rightarrow> mat_add (denoFun (fst (snd mc)) (u (fst mc) \<rho>)) (denoFun (Cond mcr) \<rho>))) + Tr (mat_mult (M_sum x) \<rho>) -
+          Tr (case x of [] \<Rightarrow> zero | mc # mcr \<Rightarrow> mat_add (denoFun (fst (snd mc)) (u (fst mc) \<rho>)) (denoFun (Cond mcr) \<rho>))"
+apply auto
+apply (induct x, auto)
+using zero_mult_r apply auto[1]
+apply(simp add:mult_allo1)
+apply(simp add:tr_allo)
+apply(simp add:mult_allo2)
+apply(simp add:tr_allo)
+apply(cut_tac  cond_aux2,auto)
+apply (drule_tac x="a" in spec)
+apply (drule_tac x="aa" in spec)
+apply (drule_tac x="b" in spec)
+apply (drule_tac x="b" in spec)
+apply (drule_tac x="aa" in spec)
+apply (drule_tac x="b" in spec)
+using fsts.intros snds.intros apply fastforce+
+done
+
+(*cond_wlp*)    
+lemma w_cond:"\<forall>a aa b aaa ba xaaa Q \<rho>. (a, aa, b) \<in> set x \<longrightarrow> (aaa, ba) \<in> Basic_BNFs.snds (a, aa, b) \<longrightarrow>
+              xaaa \<in> Basic_BNFs.fsts (aaa, ba) \<longrightarrow> wellDefined xaaa \<longrightarrow> \<rho> \<in> rhoMat \<longrightarrow>
+     Tr (mat_mult (wlp Q xaaa) \<rho>) = Tr (mat_mult Q (denoFun xaaa \<rho>)) + Tr \<rho> - Tr (denoFun xaaa \<rho>) \<Longrightarrow>
+     M_sum x = I \<Longrightarrow> \<forall>a aa b. (a, aa, b) \<in> set x \<longrightarrow> (\<forall>aaa ba. (aaa, ba) \<in> Basic_BNFs.snds (a, aa, b) \<longrightarrow>
+   (\<forall>xaaa. xaaa \<in> Basic_BNFs.fsts (aaa, ba) \<longrightarrow> wellDefined xaaa)) \<Longrightarrow> \<forall>Q \<rho>.  \<rho> \<in> rhoMat \<longrightarrow> Tr (mat_mult (case x of [] \<Rightarrow> zero
+      | mc # mcr \<Rightarrow> mat_add (uu (fst mc) (wlp Q (fst (snd mc)))) (wlp Q (Cond mcr)))  \<rho>) =
+      Tr (mat_mult Q (case x of [] \<Rightarrow> zero  | mc # mcr \<Rightarrow> mat_add (denoFun (fst (snd mc)) (u (fst mc) \<rho>)) (denoFun (Cond mcr) \<rho>))) +
+     Tr \<rho> - Tr (case x of [] \<Rightarrow> zero
+        | mc # mcr \<Rightarrow> mat_add (denoFun (fst (snd mc)) (u (fst mc) \<rho>)) (denoFun (Cond mcr) \<rho>))"
+apply(rule cond_aux)
+apply simp
+apply(cut_tac x=x in cond_aux_1,auto)
+done
+
+(*while_wlp *)
+lemma w_while_n:" wellDefined (While_n Mata Matb com Matc m) \<Longrightarrow>  
+ \<forall>Q.\<forall> \<rho>. \<rho> \<in> rhoMat \<longrightarrow> Tr (mat_mult (wlp Q com) \<rho>) = Tr (mat_mult Q (denoFun com \<rho>)) + Tr \<rho> - Tr (denoFun com \<rho>)  \<Longrightarrow>
+ \<forall>\<rho>. \<rho> \<in> rhoMat \<longrightarrow>
+       Tr (mat_mult (case num of 0 \<Rightarrow> I | Suc m \<Rightarrow> mat_add (uu Mata Q) (uu Matb (wlp (wlp Q (While_n Mata Matb com Matc m)) com))) \<rho>) =
+       Tr (mat_mult Q
+            (case num of 0 \<Rightarrow> zero | Suc m \<Rightarrow> mat_add (u Mata \<rho>) (denoFun (While_n Mata Matb com Matc m) (denoFun com (u Matb \<rho>))))) +
+       Tr \<rho> -
+       Tr (case num of 0 \<Rightarrow> zero | Suc m \<Rightarrow> mat_add (u Mata \<rho>) (denoFun (While_n Mata Matb com Matc m) (denoFun com (u Matb \<rho>))))"
+apply(induct num,auto)
+apply (smt Ident zero_mult_r)
+apply(simp add:mult_allo1)
+apply(simp add:tr_allo)
+apply(simp add:while_n_aux)
+apply(simp add:mult_allo2)
+apply(simp add:tr_allo)
+apply(subgoal_tac "(denoFun com (u Matb \<rho>))\<in>rhoMat")
+prefer 2
+apply (metis b rho)
+apply(drule_tac x="(denoFun com (u Matb \<rho>))"in spec)
+apply(drule_tac x="(case num of 0 \<Rightarrow> I | Suc m \<Rightarrow> mat_add (uu Mata Q) (uu Matb (wlp (wlp Q (While_n Mata Matb com Matc m)) com)))"in spec)
+apply(subgoal_tac "(u Matb \<rho>)\<in>rhoMat")
+prefer 2
+apply (metis rho)
+apply(drule_tac x="(u Matb \<rho>)"in spec)
+apply(simp add:while_n_aux2)
+apply(simp add:u_def)
+apply(simp add:exchange)
+by (smt Ident mult_allo1 mult_exchange tr_allo)
+
+(*  while_wlp   *)
+lemma w_while:" wellDefined (While Mata Matb com Matc ) \<Longrightarrow>
+ \<forall>Q \<rho>. \<rho> \<in> rhoMat \<longrightarrow> Tr (mat_mult (wlp Q com) \<rho>) = Tr (mat_mult Q (denoFun com \<rho>)) + Tr \<rho> - Tr (denoFun com \<rho>) \<Longrightarrow>
+    \<forall>\<rho>. \<rho> \<in> rhoMat \<longrightarrow> Tr (mat_mult (fixpoint_wlp Mata Matb com Matc Q) \<rho>)
+      = Tr (mat_mult Q (fixpoint Mata Matb com Matc \<rho>)) + Tr \<rho> - Tr (fixpoint Mata Matb com Matc \<rho>)"
+apply auto
+apply(rule aux)
+apply(rule aux1)
 apply(rule fixpoint_wlp_lemma,auto)
-apply (smt2 Ident ascend zero_mult_l fg sum_1.simps(1))
-by (metis (full_types) Ident zero_mult_l fg sum_1.simps(1))
-
-(*    Seq     *)
-lemma wlp_seq: "\<forall>Q. valid (wlp Q coma) coma Q \<Longrightarrow> \<forall>Q. valid (wlp Q comb) comb Q 
-   \<Longrightarrow> valid (wlp (wlp Q comb) coma) (coma; comb) Q"
-apply (drule_tac x = "(wlp Q comb)" in  spec)
-apply (drule_tac x = "Q" in  spec)
-apply (rule Seq, auto)
+apply(simp add:tr_allo)
+apply(cut_tac wlp_while_aux,auto)
 done
-lemma soundwp1: "wellDefined S \<Longrightarrow>\<forall> Q. valid (wlp Q S) S  Q"
-apply (induct S,auto)
-apply (cut_tac wlp_skip, auto)
-apply (cut_tac wlp_init, auto)
-apply (cut_tac wlp_utrans, auto)
-apply (cut_tac Q = Q and  coma = "S1" and comb = "S2" in wlp_seq, auto)
-apply (cut_tac wlp_cond, auto)
+
+(*\<forall> \<rho>,Q\<longrightarrow>Tr (wlp Q S)*\<rho>=Tr Q*[S](\<rho>)+ Tr \<rho>-Tr [S](\<rho>)          *)
+lemma eq:"wellDefined S\<Longrightarrow>\<forall>Q. \<forall>\<rho>. \<rho>\<in>rhoMat\<longrightarrow> Tr (mat_mult (wlp Q S) \<rho>) =Tr (mat_mult Q (denoFun S \<rho>)) +Tr \<rho>-Tr (denoFun S \<rho>)"
+apply(induct S,auto)
+apply(cut_tac w_init,auto)
+apply(cut_tac w_utrans,auto)
+apply(cut_tac Sa="S1"and Sb="S2" in w_seq,auto)
+prefer 3
+apply(cut_tac Mata="x1" and Matb="x2" and Matc="x4" and com="S" and Q="Q" in w_while_n,auto)
 defer
-apply (metis (poly_guards_query) Ident zero_mult_l eq_valid fg less_irrefl not_le sum_1.simps(1) svalid_def)
-apply(cut_tac Mata="Mat1" and Matb="Mat2" and Matc="Mat3" and com="S" and Q="Q" in wlp_while,auto)
-by (metis (poly_guards_query) Ident zero_mult_l fg order_refl sum_1.simps(1) tr_allo tr_allo1 valid_def)
+apply(cut_tac w_while,auto)
+apply(cut_tac w_cond,auto)
+done
+
+
+lemma soundwp1: "wellDefined S \<Longrightarrow>\<forall> Q. valid (wlp Q S) S  Q"
+apply(simp add:valid_def)
+apply(simp add:eq)
+done
 
 lemma WLPsound:"Q\<in>predMat\<Longrightarrow>wellDefined S\<Longrightarrow>valid (wlp Q S) S Q"
 apply(simp add: soundwp1)
 done
+
 lemma ord_wlp:"Q\<in>predMat\<Longrightarrow>P\<in>predMat\<Longrightarrow>wellDefined S\<Longrightarrow>less P (wlp Q S)\<Longrightarrow>valid P S Q"
 apply(rule_tac Pa="wlp Q S" in order,auto)
 apply(rule WLPsound)
 apply auto
 done
+
 declare uu_def[simp]
 ML_file "Quantum_Hoare_tac.ML"
 method_setup vcg = {*
@@ -366,6 +723,9 @@ method_setup vcg_simp = {*
   Scan.succeed (fn ctxt =>
     SIMPLE_METHOD' (quantum_hoare_tac ctxt (asm_full_simp_tac ctxt))) *}
 end
+
+
+
 
 
 
